new_example/calendar.go
@@ -1,6 +1,7 @@
 package main
 
 import "github.com/tchajed/marshal"
+import "github.com/goose-lang/std"
 
 type Calendar struct {
 	hash   []byte
@@ -15,6 +16,7 @@ func MarshalCalendar(enc []byte, c Calendar) []byte {
 
 func UnmarshalCalendar(s []byte) (Calendar, []byte) {
 	hash, s := marshal.ReadLenPrefixedBytes(s)
+	hash = std.BytesClone(hash)
 	eventsLen, s := marshal.ReadInt(s)
 	events, s := marshal.ReadSlice[Event](s, eventsLen, UnmarshalEvent)
 
